Move inlining back up in the compiler

compiler/backend/passes/pure_letrec_cexpScript.sml
@@ -186,19 +186,20 @@ End
     Putting it all together:
 *)
 
-Definition transform_cexp_def:
-  transform_cexp (conf:compiler_opts) e =
-    let e = init_sets e in
-    let d = distinct_cexp e in
-      if ~conf.do_pure_sort then d else
-        let s = split_all_cexp d in
-          s
-End
-
 Definition clean_cexp_def:
   clean_cexp (conf:compiler_opts) e =
     if conf.do_pure_clean then clean_all_cexp e else e
 End
+
+Definition transform_cexp_def:
+  transform_cexp (conf:compiler_opts) e =
+    let e = init_sets e in
+    let d = distinct_cexp e in
+      clean_cexp conf $ if ~conf.do_pure_sort then d else
+                          let s = split_all_cexp d in
+                            s
+End
+
 
 (*******************)
 
